reduce/WorkStealing.v
@@ -1,0 +1,52 @@
+Require Export ProcessRewrite.
+Require Export RewriteTactics.
+(** 
+< q             ▹ foreach (i ∈ [1..n]):
+                                 ∀p. recv(p); send(p, Integer);
+                               μX. ∀p. recv(p); send(p, tt); X
+               p[len slaves] ▹ μX. send(q, me); { recv(Int); send(me, Int); X
+                                                , recv(tt)
+                                                };
+               me            ▹ foreach (i ∈ [1..n]):
+                                 recv(Integer)
+             > Integer
+**)
+
+
+Inductive Message :=
+  | int
+  | id
+  | tt.
+
+Parameters me q x : pid.
+Parameters xs ps : SetVar.
+Parameters X : MuVar.
+Hypothesis H : measure xs = measure ps.
+Hypothesis G : me <> q /\ me <> x /\ q <> x.
+
+Definition worker_loop :=
+  s_send (p_sng q) (id, p_set ps); s_recv (int, p_none); s_send (p_sng me) (int, p_none); s_var X.
+
+Example WorkStealing0 :
+    [ q    [[ s_iter xs (x ~ (s_recv(id, p_sng x); 
+                              s_send (p_sng x) (int, p_none))) ]]
+    | {ps} [[ s_loop X worker_loop ]]
+    | me   [[ s_iter xs (s_recv (int, p_none)) ]]
+    ] 
+      ===> 
+    [ q    [[ s_skip ]]
+    | {ps} [[ s_loop X worker_loop ]]
+    | me   [[ s_skip ]]
+    ].
+Proof.
+  intros.
+  inst_bind 0.
+  rewrite_eq_stmt 1.
+  apply stmt_unfold_loop.
+  reduce_pair 0 1.
+  reduce_pair 0 1.
+  reduce_pair 1 2.
+  rewrite_eq_stmt 1.
+  apply stmt_fold_loop.
+  skip.
+Qed.
